day 6

problems/6/Problem6.dfy
@@ -1,9 +1,174 @@
+include "../../parser/split.dfy"
+include "../../parser/parseInt.dfy"
 module Problem6 {
+    import opened Split
+    import opened ParseInt
+    import opened Std.Collections.Seq
+
+    datatype Op = Add | Mul
+    method parseInput(input: string) returns (data: seq<seq<nat>>, ops: seq<Op>, length: nat)
+        ensures |ops| == length
+        ensures forall d :: d in data ==> |d| == length
+    {
+        var lines := splitOnBreak(input);
+        expect |lines| > 1;
+        var ops_line := split(lines[|lines|-1], " ");
+        lines := lines[..|lines|-1];
+        data := [];
+        ops := [];
+        length := 0;
+        for i := 0 to |ops_line| {
+            if Contains(ops_line[i], "+") {
+                ops := ops + [Add];
+            } else if Contains(ops_line[i], "*") {
+                ops := ops + [Mul];
+            }
+        }
+        length := |ops|;
+        print "\nops ", length;
+        for i := 0 to |lines| 
+            invariant forall d :: d in data ==> |d| == length
+            invariant |data| == i
+        {
+            var row := Map(Integer, Filter(xs => xs != "", split(lines[i], " ")));
+            print "\nrow ", i," ", |row|, " ", row;
+            expect |row| == length;
+            expect forall i: nat :: i < |row| ==> 0 < row[i];
+            data := data + [row];
+        }
+        
+    }
+
+    function transpose(vals: seq<seq<nat>>, columns: nat, rows: nat): seq<seq<nat>> 
+        requires forall d :: d in vals ==> |d| == columns
+        requires |vals| == rows 
+    {
+        seq(columns, i requires 0 <= i < columns => seq(rows, j requires 0 <= j < rows => vals[j][i]))
+    }
+
+    function add(x: nat, y: nat): nat {
+        x + y
+    }
+
+    function mul(x: nat, y: nat): nat {
+        x * y
+    }
+
     method problem6_1(input: string) returns (x: int) {
-        return 3;
+        var data, ops, length := parseInput(input);
+        // print "\n", data;
+        print "\n", ops;
+        var homework := transpose(data, length, |data|);
+        print "\n", homework;
+        x := 0;
+        expect |homework| == length;
+        for i := 0 to |homework| 
+        {
+            var res := match ops[i] {
+                case Add => FoldLeft(add, 0, homework[i])
+                case Mul => FoldLeft(mul, 1, homework[i])
+            };
+            // print "\nwhat: ", what;
+            x := x + res;
+        }
+        print "\n";
+    }
+    function maxLength<T>(xs: seq<seq<T>>): nat 
+        ensures forall d :: d in xs ==> |d| <= maxLength(xs)
+    {
+        if xs == [] then
+            0
+        else
+            var rl := maxLength(xs[1..]);
+            if |xs[0]| > rl then |xs[0]| else rl
+    }
+
+    function ToDigits(n: nat): seq<nat> {
+        if n < 10 then [n] else ToDigits(n/10)+[n%10]
+    }
+
+    method ToCephalopod(nums: seq<nat>) returns (res: seq<nat>)
+    {
+        print "\n", Map(ToDigits, nums);
+        var digits := Map(ToDigits, nums);
+        res := [];
+        var num_seqs: seq<seq<nat>> := [];
+    }
+
+    function opIndexes(s: string, i: nat, idx: seq<nat>): seq<nat> {
+        if s == [] then
+            idx 
+        else match s[0] {
+            case '+' => opIndexes(s[1..], i+1, idx+[i])
+            case '*' => opIndexes(s[1..], i+1, idx+[i])
+            case _ => opIndexes(s[1..],i+1, idx)
+        }
+    }
+
+    method parseInput2(input: string) returns (data: seq<seq<nat>>, ops: seq<Op>, length: nat)
+        ensures |ops| == length
+        ensures |data| == length
+    {
+        var lines := splitOnBreak(input);
+        expect |lines| > 1;
+        var ops_line := split(lines[|lines|-1], " ");
+        var raw_op_lines := lines[|lines|-1];
+        lines := lines[..|lines|-1];
+        data := [];
+        ops := [];
+        length := 0;
+        for i := 0 to |ops_line| {
+            if Contains(ops_line[i], "+") {
+                ops := ops + [Add];
+            } else if Contains(ops_line[i], "*") {
+                ops := ops + [Mul];
+            }
+        }
+        // print "\nraw: ", raw_op_lines;
+        var op_indexes := opIndexes(raw_op_lines, 0, []);
+        // print "\nidx, ", op_indexes;
+        length := |ops|;
+        expect |op_indexes| == |ops|;
+        for i := 0 to |ops|
+        {
+            var end:int := |raw_op_lines|;
+            if i < |ops| - 1 {
+                end := op_indexes[i+1] as int -1;
+            }
+            expect op_indexes[i] < end;
+            var partials: seq<string> := [];
+            
+            for j := op_indexes[i] to end {
+                var partial := "";
+                for k := 0 to |lines| {
+                    if 0 <= j < |lines[k]| && charInNC(lines[k][j]) {
+                        partial := partial+[lines[k][j]];
+                    }
+                }
+                partials := partials + [partial];
+            }
+            // print "\n",partials;
+            var row := Map(Integer, partials);
+            expect forall i: nat :: i < |row| ==> 0 < row[i];
+            data := data + [row];
+        }
+        expect |data| == length;
     }
 
     method problem6_2(input: string) returns (x: int) {
-        return 4;
+        var data, ops, length := parseInput2(input);
+        print "\n", data;
+        print "\n", ops;
+        x := 0;
+        for i := 0 to |data| 
+        {
+            var res := match ops[i] {
+                case Add => FoldLeft(add, 0, data[i])
+                case Mul => FoldLeft(mul, 1, data[i])
+            };
+            // print "\nwhat: ", what;
+            x := x + res;
+        }
+        print "\n";
     }
 }
