parser/parseInt.dfy
@@ -71,5 +71,5 @@ module ParseInt {
 
     export
         provides Integer
-        provides toInt, toStr, isNumString
+        provides toInt, toStr, isNumString, charInNC
 }
